theories/Sem/Deinit.v
@@ -1,0 +1,54 @@
+(*
+ * Copyright (C) BedRock Systems Inc. 2019 Gregory Malecha
+ *
+ * SPDX-License-Identifier:AGPL-3.0-or-later
+ *)
+Require Import Coq.Lists.List.
+
+From Cpp Require Import
+     Ast.
+From Cpp.Sem Require Import
+     Util Logic PLogic Semantics Wp Typing.
+
+Module Type Deinit.
+
+  Section with_resolve.
+    Context {resolve : genv}.
+    Variable ti : thread_info.
+    Variable ρ : region.
+
+    Local Notation wp := (wp (resolve:=resolve)  ti ρ).
+    Local Notation wpe := (wpe (resolve:=resolve) ti ρ).
+    Local Notation wp_lhs := (wp_lhs (resolve:=resolve) ti ρ).
+    Local Notation wp_rhs := (wp_rhs (resolve:=resolve) ti ρ).
+    Local Notation wpAny := (wpAny (resolve:=resolve) ti ρ).
+    Local Notation wpAnys := (wpAnys (resolve:=resolve) ti ρ).
+    Local Notation fspec := (fspec (resolve:=resolve)).
+
+  (** destructor lists
+   *
+   *  the opposite of initializer lists, this is just a call to the
+   *  destructors *in the right order*
+   *)
+  Parameter wpd
+    : forall {resolve : genv} (ti : thread_info) (ρ : region)
+        (cls : globname) (this : val)
+        (init : FieldOrBase * globname)
+        (Q : mpred), mpred.
+
+  Fixpoint wpds
+           (cls : globname) (this : val)
+           (dests : list (FieldOrBase * globname))
+           (Q : mpred) : mpred :=
+    match dests with
+    | nil => Q
+    | d :: ds => @wpd resolve ti ρ cls this d (wpds cls this ds Q)
+    end.
+
+  End with_resolve.
+
+End Deinit.
+
+Declare Module D : Deinit.
+
+Export D.
